src/tutorial/Imp.v
@@ -82,6 +82,7 @@ Coercion ANum : nat >-> aexp.
 
 Declare Custom Entry com.
 Declare Scope com_scope.
+Delimit Scope com_scope with com.
 
 Notation "<{ e }>" := e (at level 0, e custom com at level 99) : com_scope.
 Notation "( x )" := x (in custom com, x at level 99) : com_scope.
